new/golang/theory/interface.v
@@ -1,6 +1,6 @@
 From Perennial.goose_lang Require Import notation.
-From New.golang.theory Require Import struct typing proofmode globals.
-From New.golang.defn Require Import interface globals.
+From New.golang.theory Require Import struct typing proofmode pkg.
+From New.golang.defn Require Import interface.
 
 Set Default Proof Using "Type".
 
